% Created 2023-03-26 Sun 10:19
% Intended LaTeX compiler: pdflatex
\documentclass[11pt]{article}
\usepackage[utf8]{inputenc}
\usepackage[T1]{fontenc}
\usepackage{graphicx}
\usepackage{longtable}
\usepackage{wrapfig}
\usepackage{rotating}
\usepackage[normalem]{ulem}
\usepackage{amsmath}
\usepackage{amssymb}
\usepackage{capt-of}
\usepackage{hyperref}
\author{Yusheng Zhao}
\date{\today}
\title{HW 7}
\hypersetup{
 pdfauthor={Yusheng Zhao},
 pdftitle={HW 7},
 pdfkeywords={},
 pdfsubject={},
 pdfcreator={Emacs 28.2 (Org mode 9.6.1)}, 
 pdflang={English}}
\begin{document}

\maketitle
\tableofcontents


\section{Problem 1}
\label{sec:orgee4383a}
Following Hook's Law, we have the next system of equation.

\begin{equation}
\begin{cases}
M_{A} \frac{\partial u_{i}^{2}}{\partial t^{2}} = \lambda (w_{i-1} - u_{i})+ \lambda (v_{i}-u_{i}) \\
M_{B} \frac{\partial v_{i}^{2}}{\partial t^{2}} = \lambda (w_{i} - v_{i}) + \lambda (u_{i}-v_{i}) \\
M_{C} \frac{\partial w_{i}^{2}}{\partial t^{2}} = \lambda (v_{i} - w_{i}) + \lambda (u_{i+1}-w_{i})
\end{cases}
\end{equation}
Due to periodicity of our system, we solve with ansatz \(u_{i} = A e^{i\omega t}
e^{ik a}\), \(v_{i} = B e^{i\omega t} e^{ika}\) and, \(w_{i} = C e^{i\omega t}
e^{ika}\). we have
\begin{align}
&\begin{cases}
-M_{A} \omega^{2} u_{i} = \lambda (w_{i-1} - u_{i}) + \lambda (v_{i}-u_{i}) \\
-M_{B} \omega^{2} v_{i} = \lambda (w_{i} - v_{i}) + \lambda (u_{i}-v_{i}) \\
-M_{C} \omega^{2} w_{i} = \lambda (v_{i} - w_{i}) + \lambda (u_{i+1}-w_{i})
\end{cases}\\
&\begin{cases}
-M_{A} \omega^{2} A = \lambda (C e^{-ika} - A) + \lambda (B-A) \\
-M_{B} \omega^{2} B = \lambda (C - B) + \lambda (A-B) \\
-M_{C} \omega^{2} C = \lambda (B - C) + \lambda (Ae^{ika}-C)
\end{cases}\\
&\begin{cases}
-\frac{M_{A}}{\lambda} \omega^{2} A = (C e^{-ika} - A) + (B-A) \\
-\frac{M_{B}}{\lambda} \omega^{2} B = (C - B) + (A-B) \\
-\frac{M_{C}}{\lambda} \omega^{2} C = (B - C) + (Ae^{ika}-C)
\end{cases}\\
&\begin{pmatrix}
\frac{M_{A}}{\lambda}\omega^{2} -2 & 1 & e^{-ika} \\
1 & \frac{M_{B}}{\lambda}\omega^{2} - 2 & 1 \\
e^{ika} & 1 & -\frac{M_{C}}{\lambda} \omega^{2} - 2
\end{pmatrix}
\begin{pmatrix}
A \\ B \\ C
\end{pmatrix} = \vec{0}
\end{align}
\end{document}